operations/Expression_Like_Strong.thy
@@ -2,40 +2,54 @@ theory Expression_Like_Strong
   imports Expression_Like
 begin
 
-axiomatization where
+locale Expression_Strong = Expression +
+  fixes Ebd :: "'bd rel"
+  assumes
   Ector_fresh_surj: "\<And>A e. |A::'a set| <o |UNIV :: 'a::var set| \<Longrightarrow> 
     \<exists>u. GVrs2 u \<inter> A = {} \<and> e = Ector u" and
   Ector_eqI: "\<And>x y.
    (\<exists>\<sigma> :: 'a :: var \<Rightarrow> 'a. bij \<sigma> \<and> |supp \<sigma>| <o |UNIV :: 'a set| \<and>
      id_on (\<Union> (EVrs ` GSupp1 x) - GVrs2 x) \<sigma> \<and> Gren id \<sigma> (Gmap (Eperm \<sigma>) id x) = y) \<Longrightarrow> Ector x = Ector y" and
-  E_coinduct: "\<And>P (g :: 'a::var E \<Rightarrow> 'a E) h e. (\<And>e. P e \<Longrightarrow> g e = h e \<or>
+  E_coinduct: "\<And>P (g :: 'e \<Rightarrow> 'e) h e. (\<And>e. P e \<Longrightarrow> g e = h e \<or>
        (\<exists>u. g e = Ector (Gmap g g u) \<and> h e = Ector (Gmap h h u) \<and>
          (\<forall>e \<in> GSupp1 u. P e) \<and> (\<forall>e \<in> GSupp2 u. P e))) \<Longrightarrow>
-         P e \<Longrightarrow> g e = h e" 
+         P e \<Longrightarrow> g e = h e"
+  and Ebd_infinite_regular_card_order: "infinite_regular_card_order Ebd"
+  and Ebd_le: "Ebd \<le>o |UNIV :: 'a::var set|"
   and EVrs_bd:
-  "\<And>x. |EVrs (x :: 'a :: var E)| <o Gbd"
+  "\<And>x. |EVrs (x :: 'e)| <o Ebd"
+begin
 
 lemma Ector_inject: "\<And>x y. (Ector x = Ector y) =
    (\<exists>\<sigma> :: 'a :: var \<Rightarrow> 'a. bij \<sigma> \<and> |supp \<sigma>| <o |UNIV :: 'a set| \<and>
      id_on (\<Union> (EVrs ` GSupp1 x) - GVrs2 x) \<sigma> \<and> Gren id \<sigma> (Gmap (Eperm \<sigma>) id x) = y)"
   using Ector_eqI Ector_eqD by metis
 
-consts \<eta> :: "'a1 :: var \<Rightarrow> ('a1, 'a2 :: var, 'x1, 'x2) G"
-consts \<eta>' :: "'a1 :: var \<Rightarrow> ('a1, 'a2 :: var, 'x1, 'x2) G"
+lemma EVrs_bound[simp]: "|EVrs (x :: 'e)| <o |UNIV :: 'a set|"
+  by (rule ordLess_ordLeq_trans[OF EVrs_bd Ebd_le])
 
-axiomatization where
-  eta_inversion: "\<And>\<delta>1 \<delta>2 f1 f2 u a. |supp \<delta>1| <o |UNIV::'a1 set| \<Longrightarrow> |supp \<delta>2| <o |UNIV::'a2 set| \<Longrightarrow>
-   Gsub \<delta>1 \<delta>2 (Gmap f1 f2 u) = (\<eta> a :: ('a1::var, 'a2 :: var, 'x1, 'x2) G) \<Longrightarrow> \<exists>y. u = \<eta> y"
-  and eta_natural: "\<And>\<delta>1 \<delta>2 f1 f2 a. |supp \<delta>1| <o |UNIV::'a1 set| \<Longrightarrow> |supp \<delta>2| <o |UNIV::'a2 set| \<Longrightarrow>
-   Gsub \<delta>1 \<delta>2 (Gmap f1 f2 (\<eta> a :: ('a1::var, 'a2 :: var, 'x1, 'x2) G)) = \<eta> (\<delta>1 a)"
-  and eta_mem: "\<And>a. a \<in> GVrs1 (\<eta> a :: ('a1::var, 'a2 :: var, 'x1, 'x2) G)"
-  and eta'_inversion: "\<And>\<delta>1 \<delta>2 f1 f2 u a. |supp \<delta>1| <o |UNIV::'a1 set| \<Longrightarrow> |supp \<delta>2| <o |UNIV::'a2 set| \<Longrightarrow>
-   Gsub \<delta>1 \<delta>2 (Gmap f1 f2 u) = \<eta>' a \<Longrightarrow> \<exists>y. u = \<eta>' y"
-  and eta'_natural: "\<And>\<delta>1 \<delta>2 f1 f2 a. |supp \<delta>1| <o |UNIV::'a1 set| \<Longrightarrow> |supp \<delta>2| <o |UNIV::'a2 set| \<Longrightarrow>
-   Gsub \<delta>1 \<delta>2 (Gmap f1 f2 (\<eta>' a :: ('a1::var, 'a2 :: var, 'x1, 'x2) G)) = \<eta>' (\<delta>1 a)"
-  and eta'_mem: "\<And>a. a \<in> GVrs1 (\<eta>' a :: ('a1::var, 'a2 :: var, 'x1, 'x2) G)"
-  and eta_inj: "\<And>a a'. \<eta> a = \<eta> a' \<Longrightarrow> a = a'"
-  and eta'_inj: "\<And>a a'. \<eta>' a = \<eta>' a' \<Longrightarrow> a = a'"
-  and eta_distinct: "\<And>a a'. \<eta> a \<noteq> \<eta>' a'"
+lemma GVrs2_bound[simp]: "|GVrs2 (u::('a :: var, 'a, 'e, 'e) G)| <o |UNIV :: 'a set|"
+  by (rule ordLess_ordLeq_trans[OF G.Vrs_bd(2) large'])
+
+lemma Ector_fresh_inject:
+  assumes "GVrs2 x \<inter> A = {}" "GVrs2 y \<inter> A = {}" "|A :: 'a::var set| <o |UNIV :: 'a set|"
+  shows "(Ector x = Ector y) = (\<exists>\<sigma>. bij \<sigma> \<and> |supp \<sigma>| <o |UNIV :: 'a set| \<and> imsupp \<sigma> \<inter> A = {}
+    \<and> id_on (\<Union> (EVrs ` GSupp1 x) - GVrs2 x) \<sigma> \<and> Gren id \<sigma> (Gmap (Eperm \<sigma>) id x) = y)"
+  unfolding Ector_inject
+  apply (rule iffI; elim exE conjE)
+  subgoal for \<sigma>
+    apply (insert ex_avoiding_bij[of \<sigma> "(\<Union> (EVrs ` GSupp1 x) - GVrs2 x)" "GVrs2 x" A])
+    apply (drule meta_mp; simp add: UN_bound card_of_minus_bound ordLess_ordLeq_trans[OF G.Supp_bd(1) large'] ordLess_ordLeq_trans[OF G.Vrs_bd(2) large'] assms)+
+    apply (elim exE conjE)
+    subgoal for \<tau>
+      apply (auto simp: G.Vrs_Map Gren_def intro!: exI[of _ \<tau>] trans[OF G.Sb_cong arg_cong[where f="Gsub _ _", OF G.Map_cong]] Eperm_cong)
+      using G.Vrs_Map(2) G.Vrs_Sb(2) assms(2) imageI supp_id_bound apply blast
+      apply (smt (verit, ccfv_threshold) Diff_iff G.Vrs_Map(2) G.Vrs_Sb(2) UN_I assms(2) disjoint_iff_not_equal id_on_eq imageI supp_id_bound)
+      done
+    done
+  apply blast
+  done
+
+end
 
 end
